Cleaning up lemmas and names

AVL Tree.v
@@ -3,19 +3,37 @@ Require Import Coq.Numbers.Natural.Peano.NPeano.
 
 Definition blt_nat n1 n2 :=
 	negb (ble_nat n2 n1).
+	
+Lemma not_lt_S : forall n m,
+	(~ n < m) -> (~ S n < S m).
+Proof.
+	intros. unfold not in *. intros. apply H. omega.
+Qed.
 
-Definition bgt_nat n1 n2 :=
-	negb (ble_nat n1 n2).
+Lemma blt_nat_false : forall n m,
+	blt_nat n m = false -> ~(n < m).
+Proof. 
+	induction n. 
+		intros. destruct m. 
+			omega. 
+			inversion H. 
+		intros. destruct m.
+			omega. 
+			apply not_lt_S. apply IHn. replace (blt_nat n m = false) with (blt_nat (S n) (S m) = false). apply H.
+				unfold blt_nat. simpl. reflexivity.
+Qed.
 
-Fixpoint contains elem l :=
-	match l with
-	| [] => false
-	| x::xs =>
-		match beq_nat elem x with
-		| true => true
-		| false => contains elem xs
-		end
-	end.
+Lemma blt_nat_true : forall n m,
+	blt_nat n m = true -> n < m.
+Proof.
+	induction n.
+		destruct m.
+			intros. unfold blt_nat in H. simpl in H. inversion H.
+			intros. omega.
+		destruct m.
+			intros. unfold blt_nat in H. simpl in H. inversion H.
+			intros. apply lt_n_S. apply IHn. unfold blt_nat in *. apply negb_true_iff. apply negb_true_iff in H. simpl in H. assumption.
+Qed.
 
 Fixpoint first l :=
 	match l with
@@ -36,22 +54,17 @@ Inductive tree: Type :=
 	        (* Value -> Left -> Right *)
 
 Inductive sorted : list nat -> Prop :=
-	| empty : sorted []
-	| single : forall n, sorted [n]
-	| more : forall n m xs, n <= m -> sorted (m::xs) -> sorted (n::m::xs).
+	| s_nil : sorted []
+	| s_single : forall n, sorted [n]
+	| s_cons : forall n m xs, n <= m -> sorted (m::xs) -> sorted (n::m::xs).
 
-Inductive bst : tree -> Prop :=
-	| bst_leaf : bst leaf
-	| bst_node : forall val rVal lVal llT lrT rlT rrT, 
-		ble_nat lVal val = true -> bgt_nat rVal val = true -> bst (node lVal llT lrT) -> 
-		bst (node rVal lrT rrT) -> bst (node val (node lVal llT lrT) (node rVal rlT rrT))
-	| bst_node_leaf : forall val lVal llT lrT, 
-		ble_nat lVal val = true -> bst (node lVal llT lrT) -> 
-		bst (node val (node lVal llT lrT) leaf)
-	| bst_leaf_node : forall val rVal rlT rrT, 
-		bgt_nat rVal val = true -> bst (node rVal rlT rrT) -> 
-		bst (node val leaf (node rVal rlT rrT))
-	| bst_leaf_leaf : forall val, bst (node val leaf leaf).
+	
+Fixpoint max n m {struct n} : nat :=
+  match n, m with
+    | O, _ => m
+    | S n', O => n
+    | S n', S m' => S (max n' m')
+  end.
 
 Fixpoint height (t: tree) :=
 	match t with
@@ -110,25 +123,13 @@ Fixpoint balance (t : tree) :=
 Definition insert val t :=
 	balance (add val t).
 
-Fixpoint search (searchFor : nat) (t : tree) :=
-	match t with
-	| leaf => None
-	| node val leftChild rightChild => 
-		match beq_nat val searchFor with
-		| true => Some t
-		| false => 
-			match ble_nat searchFor val with
-			| true => search searchFor leftChild
-			| false => search searchFor rightChild
-			end
-		end
-	end.
 
 Fixpoint inorder (t: tree) :=
 	match t with
 	| leaf => []
 	| node val leftChild rightChild => (inorder leftChild)++val::(inorder rightChild)
 	end.
+
 
 Lemma empty_app : forall (l1: list nat) (l2 : list nat),
 	 [] = l1 ++ l2 -> l1 = [] /\ l2 = [].
@@ -148,17 +149,17 @@ Lemma cons_sorted : forall n l,
 	sorted (n::l) -> sorted l.
 Proof. 
 	intros. inversion H. 
-		apply empty. 
+		apply s_nil. 
 		subst. apply H3.
 Qed.
 
-Lemma cons_sorted_simpl : forall n l,
+Lemma sorted_cons : forall n l,
 	n <= first l -> sorted l -> sorted(n::l).
 Proof.
 	intros. remember (n::l). induction H0.
-	subst. apply single.
-	subst. apply more. apply H. apply single.
-	subst. apply more. apply H. apply more. apply H0. apply H1.
+	subst. apply s_single.
+	subst. apply s_cons. apply H. apply s_single.
+	subst. apply s_cons. apply H. apply s_cons. apply H0. apply H1.
 Qed.
 
 Lemma first_is_first : forall (m: nat) a xs xs',
@@ -171,31 +172,21 @@ Lemma app_sorted : forall l1 l2,
 	last l1 <= first l2 -> sorted l1 -> sorted l2 -> sorted(l1++l2).
 Proof. 
 	intros. induction H0. simpl in *. assumption.
-	destruct l2. simpl in *. apply single. apply more. assumption. assumption.
-	simpl. apply more. assumption. apply IHsorted. assumption.
+	destruct l2. simpl in *. apply s_single. simpl. apply s_cons. assumption. assumption.
+	simpl. apply s_cons. assumption. apply IHsorted. assumption.
 Qed.
 
-Lemma last_is_last : forall a l1 l2,
-	last(a::l1) <= first l2 -> last l1 <= first l2.
+Lemma last_cons : forall e l,
+	l <> [] -> last (e::l) = last l.
 Proof.
-	intros. induction l1. 
-		simpl. omega.
-		apply H.
+	intros. induction l.
+		apply ex_falso_quodlibet. apply H. reflexivity.
+		destruct l.
+			reflexivity.
+			simpl. reflexivity.
 Qed.
 
-Lemma last_cons : forall a l1 l2 x xs,
-	l1 = x::xs -> last l1 <= first l2 -> a <= first l1 -> last(a::l1) <= first l2.
-Proof.
-	intros. induction l2.
-		simpl in H, H0. destruct l1.
-			inversion H1. simpl. omega.
-			simpl in H1. inversion H0. auto. 
-		destruct l1.
-			inversion H1. simpl in *. omega. 
-			apply H0.
-Qed.
-
-Lemma list_property : forall x y l,
+Lemma s_cons_rev : forall x y l,
 	sorted(x::y::l) -> x <= y.
 Proof.
 	intros. inversion H. subst. apply H2. 
@@ -209,196 +200,57 @@ Proof.
 		simpl in H0. unfold not in H. destruct l2.
 			apply ex_falso_quodlibet. apply H. reflexivity.
 			simpl in IHl1. destruct l1.
-				simpl in *. apply list_property in H0. apply H0.
-				simpl in H0. apply last_cons with (x:=n0)(xs:=l1). 
-					reflexivity. 
-					apply IHl1. simpl in *. apply cons_sorted in H0. apply H0. 
-					apply list_property in H0. apply H0.
+				simpl in *. apply s_cons_rev in H0. apply H0.
+				simpl in H0. rewrite last_cons. apply IHl1. simpl in *. apply cons_sorted in H0. apply H0. 
+					apply s_cons_rev in H0. congruence.
 Qed.
 
-Lemma sorted_app_1 : forall l1 l2,
+Lemma sorted_app_l1 : forall l1 l2,
 	sorted (l1++l2) -> sorted (l1).
 Proof.
 	 intros. remember (l1++l2). generalize dependent l1. induction H. 
-	 	intros. apply empty_app in Heql. inversion Heql. rewrite H. apply empty.
+	 	intros. apply empty_app in Heql. inversion Heql. rewrite H. apply s_nil.
 	 	destruct l1.
-	 		intros. apply empty.
-	 		intros. simpl in Heql. inversion Heql. rewrite <- H0. apply empty_app in H1. inversion H1. rewrite H. apply single.
+	 		intros. apply s_nil.
+	 		intros. simpl in Heql. inversion Heql. rewrite <- H0. apply empty_app in H1. inversion H1. rewrite H. apply s_single.
 	 	intros.
 	 	destruct l1. 
-	 		apply empty.
+	 		apply s_nil.
 	 		simpl in Heql. inversion Heql. subst. destruct l1.
-	 			apply single.
-	 			apply more. inversion H3. rewrite <- H2. assumption. apply IHsorted. assumption.
+	 			apply s_single.
+	 			apply s_cons. inversion H3. rewrite <- H2. assumption. apply IHsorted. assumption.
 Qed.
 
-Lemma cons_sorted_rev : forall l n,
-	sorted(l++[n]) -> sorted l.
+Lemma sorted_app_l2 : forall l1 l2,
+	sorted (l1++l2) -> sorted l2.
 Proof.
-	intros. inversion H. destruct l. inversion H1. inversion H1. destruct l. 
-		apply empty.
-		inversion H1. destruct l. inversion H3. inversion H3. destruct l.
-			apply empty.
-			inversion H0. subst. destruct l.
-				apply single. 
-				apply more. simpl in H. apply list_property in H. 
-				apply H. simpl in H. apply sorted_app_1 with (l1:=n1::n0::l)(l2:=[n]) in H. 
-				apply cons_sorted in H. apply H.
+	intros. remember (l1++l2). generalize dependent l1. induction H.
+		intros. apply empty_app in Heql. inversion Heql. rewrite H0. apply s_nil.
+		destruct l1.
+			intros. simpl in Heql. rewrite <- Heql. apply s_single.
+			intros. simpl in Heql. inversion Heql. apply empty_app in H1. inversion H1. subst. apply s_nil.
+		intros. destruct l2.  
+ 				 apply s_nil.
+ 				 destruct l1.
+ 				 	simpl in *. rewrite <- Heql. apply s_cons. assumption. assumption.
+ 				 	inversion Heql. subst. simpl in *. inversion Heql. apply IHsorted with (l1:=l1). assumption.
 Qed.
-
-Lemma concat'_app_sorted : forall n a l1,
-	sorted (n :: l1 ++ [a]) -> sorted (n :: l1).
-Proof.
-	intros. induction l1.
-		apply single.
-		apply more. simpl in H. apply cons_sorted_rev with (l:=n::a0::l1)(n:=a) in H. apply list_property in H. apply H.
-		simpl in H. apply cons_sorted_rev with (l:=n::a0::l1)(n:=a) in H. apply cons_sorted in H. apply H. 
-Qed.
-
-Lemma concat_app_sorted : forall n l1 l2,
-	sorted (n :: l1 ++ l2) -> sorted (n::l1).
-Proof.
-	intros. generalize dependent l1. induction l2. 
-		intros. rewrite app_nil_r in H. apply H. 
-		intros. assert (sorted (n::l1 ++ [a])). apply IHl2. rewrite <- app_assoc. apply H. 
-		apply concat'_app_sorted in H0. apply H0. 
-Qed.
-
-Lemma concat_app_sorted' : forall n l1 l2,
-	sorted (l1 ++ n::l2) -> sorted (n::l2).
-Proof.
-	intros. induction l1. 
-		simpl in H.  apply H. 
-		apply IHl1. simpl in H. apply cons_sorted in H. apply H. 
-Qed.
-
 
 Lemma sorted_app: forall l1 l2,
 	l2 <> [] -> sorted(l1++l2) -> sorted l1 /\ sorted l2 /\ last l1 <= first l2.
 Proof. 
 	intros. split.  
 		destruct l1. 
-			apply empty.
-			simpl in H. apply concat_app_sorted in H0. apply H0.
+			apply s_nil.
+			simpl in H. apply sorted_app_l1 in H0. apply H0.
 		split.
 			destruct l2.
-				apply empty.
-				apply concat_app_sorted' in H0. apply H0.  
+				apply s_nil.
+				apply sorted_app_l2 in H0. apply H0.  
 			apply sorted_property in H0. apply H0. apply H.
 Qed.
 
-Lemma last_app : forall l n,
-	last (l ++ [n]) = last ([n]).
-Proof.
-	intros. simpl. induction l. 
-		reflexivity.
-		simpl in *. rewrite IHl. remember (l++[n]) as obviouslynonemptylist. destruct obviouslynonemptylist.
-			subst. simpl in *. destruct l. inversion Heqobviouslynonemptylist. inversion Heqobviouslynonemptylist. 
-			reflexivity.
-Qed.
-
-Lemma last_cons_nonempty : forall e l,
-	l <> [] -> last (e::l) = last l.
-Proof.
-	intros. induction l.
-		apply ex_falso_quodlibet. apply H. reflexivity.
-		destruct l.
-			reflexivity.
-			simpl. reflexivity.
-Qed.
-
-Lemma last_app_l : forall l1 l2 e,
-	last (l1++e::l2) = last (e::l2).
-Proof.
-	intros. induction l1. 
-		reflexivity. 
-		destruct l1. 
-			reflexivity. 
-			simpl. remember (l1 ++ e::l2) as nonemptylist. destruct nonemptylist.
-				destruct l1. inversion Heqnonemptylist. inversion Heqnonemptylist.
-				rewrite Heqnonemptylist. replace ((n::l1)++e::l2) with (n::l1++e::l2) in IHl1. 
-				rewrite last_cons_nonempty with (e:=n)(l:=l1++e::l2) in IHl1. 
-				replace (match l2 with | [] => e | _::_ => last l2 end) with (last (e::l2)). rewrite <- IHl1. reflexivity.
-				simpl. reflexivity.
-				unfold not. intros. destruct l1. inversion H. inversion H.
-				reflexivity.
-Qed.
-
-Lemma last_lt : forall t e n,
-	last (e::inorder t) <= n -> last (inorder t) <= n.
-Proof.
-	intros. induction t.
-		simpl. omega.
-		remember (inorder (node n0 t1 t2)) as list. destruct list.
-			simpl. omega.
-			rewrite last_cons_nonempty in H. apply H. unfold not. intros. inversion H0.
-Qed.
-
-Lemma inorder_add_nonempty : forall n t,
-	inorder (add n t) <> [].
-Proof.
-	intros. induction t. 
-		simpl. unfold not. intros. inversion H.
-		simpl. remember (ble_nat n n0). destruct b. 
-			simpl. unfold not. intros. remember (inorder (add n t1)). destruct l. inversion H. inversion H. 
-			simpl. unfold not. intros. remember (inorder t1). destruct l. inversion H. inversion H.
-Qed.
-
-Lemma last_first_sorted : forall n m t,
-	true = ble_nat n m -> last (inorder t) <= m -> last (inorder (add n t)) <= m.
-Proof.
-	intros. induction t. 
-		simpl. symmetry in H. apply ble_nat_true in H. apply H. 
-		simpl. remember (ble_nat n n0) as add. destruct add.
-			simpl in *. rewrite last_app_l in *. apply H0. 
-			simpl in *. rewrite last_app_l in *. rewrite last_cons_nonempty. 
-			apply IHt2. apply last_lt in H0. apply H0. apply inorder_add_nonempty. 
-Qed.
-
-Lemma sorted_last: forall val leftChild rightChild,
-	sorted (inorder (node val leftChild rightChild)) -> last (inorder leftChild ++ val::inorder rightChild) = last (val::inorder rightChild).
-Proof.
-	intros. inversion H. remember (inorder leftChild). destruct l. inversion H1. inversion H1.
-	remember (inorder leftChild). destruct l. inversion H1. reflexivity. inversion H1. destruct l. inversion H3. inversion H3.
-	remember (inorder leftChild). destruct l. rewrite H0. simpl. reflexivity. remember (inorder rightChild). destruct l0. rewrite H0. 
-	rewrite last_app_l. reflexivity. rewrite H0. rewrite last_app_l. reflexivity.
-Qed.
-
-
-Lemma first_app : forall l1 l2,
-	l1 <> [] -> first (l1 ++ l2) = first l1.
-Proof.
-	intros. destruct l1.
-		congruence.
-		reflexivity.
-Qed.
-
-Lemma inorder_add_property : forall n m t,
-	sorted (n::inorder t) -> m > n -> n <= first (inorder (add m t)).
-Proof.
-	intros. induction t.
-		simpl. omega.
-		simpl. remember (ble_nat m n0). destruct b.
-			simpl. rewrite first_app.  apply IHt1. simpl in H. apply sorted_app with (l1:=n::inorder t1) in H. inversion H. apply H1. 
-			congruence. apply inorder_add_nonempty.
-			destruct t1.
-				simpl in *. apply list_property in H. apply H. 
-				simpl in *. rewrite first_app. apply sorted_app with (l1:=n::(inorder t1_1 ++ n1::inorder t1_2)) in H. inversion H.
-				remember (inorder t1_1). destruct l. simpl in *. 
-				apply list_property in H1. assumption.
-				simpl in *. apply list_property in H1. assumption.
-				congruence. destruct (inorder t1_1). simpl. congruence. simpl. congruence.
-Qed.
-
-Lemma last_cons_le : forall n m l,
-	last (n::l) <= m -> last l <= m.
-Proof.
-	intros. induction l.
-		simpl. omega.
-		simpl in *. apply H. 
-Qed.
-
-Lemma bad_matching_is_bad : forall e1 (e2:nat) l1 (l2: list nat),
+Lemma obvious_match : forall e1 (e2:nat) l1 (l2: list nat),
 	l2 <> [] -> 
 	match l1++l2 with 
 				| [] => e1 
@@ -412,13 +264,94 @@ Proof.
 		reflexivity.
 Qed.
 
+Lemma last_app : forall l1 l2,
+	l2 <> [] -> last (l1 ++ l2) = last l2.
+Proof.
+	intros. induction l1.
+		reflexivity.
+		simpl in *. rewrite obvious_match. apply IHl1. assumption.			
+Qed.
+
+Lemma first_app : forall l1 l2,
+	l1 <> [] -> first (l1 ++ l2) = first l1.
+Proof.
+	intros. destruct l1.
+		congruence.
+		reflexivity.
+Qed.
+
+Lemma last_lt : forall t e n,
+	last (e::inorder t) <= n -> last (inorder t) <= n.
+Proof.
+	intros. induction t.
+		simpl. omega.
+		remember (inorder (node n0 t1 t2)) as list. destruct list.
+			simpl. omega.
+			rewrite last_cons in H. apply H. unfold not. intros. inversion H0.
+Qed.
+
+Lemma inorder_add_nonempty : forall n t,
+	inorder (add n t) <> [].
+Proof.
+	intros. induction t. 
+		simpl. unfold not. intros. inversion H.
+		simpl. remember (ble_nat n n0). destruct b. 
+			simpl. unfold not. intros. remember (inorder (add n t1)). destruct l. inversion H. inversion H. 
+			simpl. unfold not. intros. remember (inorder t1). destruct l. inversion H. inversion H.
+Qed.
+
+Lemma add_le : forall n m t,
+	true = ble_nat n m -> last (inorder t) <= m -> last (inorder (add n t)) <= m.
+Proof.
+	intros. induction t. 
+		simpl. symmetry in H. apply ble_nat_true in H. apply H. 
+		simpl. remember (ble_nat n n0) as add. destruct add.
+			simpl in *. rewrite last_app in *; try apply H0; congruence.
+			simpl in *. rewrite last_app in *; try rewrite last_cons; 
+			try apply IHt2; try apply last_lt in H0; try assumption; try congruence. apply inorder_add_nonempty. 
+Qed.
+
+Lemma sorted_last: forall val leftChild rightChild,
+	sorted (inorder (node val leftChild rightChild)) -> last (inorder leftChild ++ val::inorder rightChild) = last (val::inorder rightChild).
+Proof.
+	intros. inversion H. remember (inorder leftChild). destruct l. inversion H1. inversion H1.
+	remember (inorder leftChild). destruct l. inversion H1. reflexivity. inversion H1. destruct l. inversion H3. inversion H3.
+	remember (inorder leftChild). destruct l. rewrite H0. simpl. reflexivity. remember (inorder rightChild). destruct l0. rewrite H0. 
+	rewrite last_app. reflexivity. congruence. rewrite H0. rewrite last_app. reflexivity. congruence.
+Qed.
+
+Lemma inorder_add_property : forall n m t,
+	sorted (n::inorder t) -> m > n -> n <= first (inorder (add m t)).
+Proof.
+	intros. induction t.
+		simpl. omega.
+		simpl. remember (ble_nat m n0). destruct b.
+			simpl. rewrite first_app.  apply IHt1. simpl in H. apply sorted_app with (l1:=n::inorder t1) in H. inversion H. apply H1. 
+			congruence. apply inorder_add_nonempty.
+			destruct t1.
+				simpl in *. apply s_cons_rev in H. apply H. 
+				simpl in *. rewrite first_app. apply sorted_app with (l1:=n::(inorder t1_1 ++ n1::inorder t1_2)) in H. inversion H.
+				remember (inorder t1_1). destruct l. simpl in *. 
+				apply s_cons_rev in H1. assumption.
+				simpl in *. apply s_cons_rev in H1. assumption.
+				congruence. destruct (inorder t1_1). simpl. congruence. simpl. congruence.
+Qed.
+
+Lemma last_cons_le : forall n m l,
+	last (n::l) <= m -> last l <= m.
+Proof.
+	intros. induction l.
+		simpl. omega.
+		simpl in *. apply H. 
+Qed.
+
 Lemma last_inorder : forall n m x t,
 	 last (inorder (add n t)) <= m -> last (x :: inorder t) <= m -> last (x :: inorder (add n t)) <= m.
 Proof.
 	intros. induction t.
 		simpl in *. apply H. 
 		simpl in *. remember (ble_nat n n0). destruct b; 
-			simpl in *; rewrite bad_matching_is_bad in *; rewrite last_app_l in *; try assumption; congruence.
+			simpl in *; rewrite obvious_match in *; rewrite last_app in *; try assumption; congruence.
 Qed.
 
 Lemma last_add : forall n m t,
@@ -427,52 +360,22 @@ Proof.
 	intros. induction t.
 		assumption.
 		simpl. remember (ble_nat n n0). destruct b.
-			simpl in *. rewrite last_app_l. rewrite last_app_l in H0. assumption.
-			simpl in *. rewrite last_app_l. rewrite last_app_l in H0. apply last_inorder. apply IHt2. apply last_cons_le in H0. apply H0. apply H0.
+			simpl in *. rewrite last_app in *; try assumption; congruence.
+			simpl in *. rewrite last_app in *. apply last_inorder. apply IHt2. apply last_cons_le in H0. assumption. assumption. 
+			congruence. congruence. congruence.
 Qed.
 
-Theorem add_preserves_bst': forall n t,
+Theorem add_preserves_bst: forall n t,
 	sorted (inorder t) -> sorted (inorder (add n t)).
 Proof.
 	intros. induction t. 
-		Case "leaf". apply single.
+		Case "leaf". simpl. apply s_single.
 		Case "node". simpl in H. apply sorted_app in H. inversion H. inversion H1. simpl. 
 			remember (ble_nat n n0) as add. destruct add. 
-				simpl. apply app_sorted; simpl; try apply last_first_sorted; try assumption. apply IHt1. assumption. 
+				simpl. apply app_sorted; simpl; try apply add_le; try assumption. apply IHt1. assumption. 
 				simpl. apply app_sorted. simpl in *. apply H3. assumption. 
-				apply cons_sorted_simpl. apply inorder_add_property. apply H2. symmetry in Heqadd. apply ble_nat_false in Heqadd. omega. 
+				apply sorted_cons. apply inorder_add_property. apply H2. symmetry in Heqadd. apply ble_nat_false in Heqadd. omega. 
 				apply IHt2. apply cons_sorted in H2. apply H2. congruence. 
-Qed.
-
-Lemma not_lt_S : forall n m,
-	(~ n < m) -> (~ S n < S m).
-Proof.
-	intros. unfold not in *. intros. apply H. omega.
-Qed.
-
-Lemma blt_nat_false : forall n m,
-	blt_nat n m = false -> ~(n < m).
-Proof. 
-	induction n. 
-		intros. destruct m. 
-			omega. 
-			inversion H. 
-		intros. destruct m.
-			omega. 
-			apply not_lt_S. apply IHn. replace (blt_nat n m = false) with (blt_nat (S n) (S m) = false). apply H.
-				unfold blt_nat. simpl. reflexivity.
-Qed.
-
-Lemma blt_nat_true : forall n m,
-	blt_nat n m = true -> n < m.
-Proof.
-	induction n.
-		destruct m.
-			intros. unfold blt_nat in H. simpl in H. inversion H.
-			intros. omega.
-		destruct m.
-			intros. unfold blt_nat in H. simpl in H. inversion H.
-			intros. apply lt_n_S. apply IHn. unfold blt_nat in *. apply negb_true_iff. apply negb_true_iff in H. simpl in H. assumption.
 Qed.
 
 Theorem balance_inorder : forall t,
@@ -488,8 +391,13 @@ Proof.
 				SSCase "t2 = Node". remember (blt_nat (height t2_1) (height t2_2)) as height2. destruct height2.
 					SSSCase "height2 = true". simpl. repeat rewrite <- app_assoc. simpl. reflexivity. 
 					SSSCase "height2 = false". destruct t2_1.
-						SSSSCase "t2_1 = Leaf". simpl in Heqheight2. destruct t2_2. simpl in *. omega. simpl in Heqheight2. 
-							symmetry in Heqheight2. apply blt_nat_false in Heqheight2. omega.
+						SSSSCase "t2_1 = Leaf". simpl in Heqheight2. destruct t2_2. simpl in *. 
+							remember (height t1). destruct n1. inversion Heqheight1. destruct n1; inversion Heqheight1.
+							simpl in Heqheight2. 
+							symmetry in Heqheight2. apply blt_nat_false in Heqheight2. 
+							remember (max (height t2_2_1) (height t2_2_2)). destruct n2. 
+								unfold not in Heqheight2. apply ex_falso_quodlibet. apply Heqheight2. omega. 
+								unfold not in Heqheight2. apply ex_falso_quodlibet. apply Heqheight2. omega. 
 						SSSSCase "t2_1 = Node". simpl. repeat rewrite <- app_assoc. reflexivity.
 			SCase "height1 = S n". destruct height1.
 				SSCase "height1' = 0". simpl. rewrite IHt1. rewrite IHt2. reflexivity.
@@ -513,150 +421,5 @@ Qed.
 Theorem insert_preserves_bst : forall n t,
 	sorted (inorder t) -> sorted (inorder (insert n t)).
 Proof.
-	intros. unfold insert. rewrite <- balance_inorder. apply add_preserves_bst'. assumption. 
-Qed.
-
-(*induction t. 
-		Case "t Leaf". simpl. apply single.
-		Case "t Node". simpl in H. apply sorted_app in H. inversion H. inversion H1. unfold insert. simpl in *. remember (ble_nat n n0) as add. 
-		destruct add. 
-			SCase "Add left tree". simpl. remember (height (add n t1) + 2 - height t2) as height1. destruct height1.
-				SSCase "height1 = 0". destruct t2. 
-					SSSCase "t2 Leaf". simpl. apply empty.
-					SSSCase "t2 Node". remember (height t2_1 + 2 - height t2_2) as height2. destruct height2.
-						SSSSCase "height2 = 0". destruct t2_1.
-							SSSSSCase "t2_1 Leaf". apply empty.
-							SSSSSCase "t2_1 Node". simpl. apply app_sorted. 
-								SSSSSSCase "app_sorted 1". simpl in *. destruct t2_1_1.
-									SSSSSSSCase "t2_1_1 Leaf". simpl in *. rewrite last_app. simpl. apply list_property in H2. apply H2. 
-									SSSSSSSCase "t2_1_1 Node". 
-										simpl. rewrite last_app_l. 
-										replace (n0 :: inorder t2_1_1_1 ++ n3 :: inorder t2_1_1_2) 
-											with ((n0 :: inorder t2_1_1_1) ++ n3 :: inorder t2_1_1_2).
-											rewrite last_app_l with (l1:=n0::inorder t2_1_1_1). 
-											apply cons_sorted in H2.
-											apply sorted_app in H2. 
-												inversion H2. subst. apply sorted_app in H4. 
-													inversion H4.
-													apply sorted_last in H6. inversion H7. simpl in H9. rewrite <- H6. apply H9. 
-												congruence.
-											congruence.
-										reflexivity.
-								SSSSSSCase "app_sorted 2". apply app_sorted. 
-									SSSSSSSCase "app_sorted 2_1". simpl. apply last_add. 
-										symmetry in Heqadd. apply ble_nat_true in Heqadd. assumption. assumption.
-									SSSSSSSCase "app_sorted 2_2". apply add_preserves_bst'. assumption.
-									SSSSSSSCase "app_sorted 2_3". simpl in H2. 
-										replace (n0 :: (inorder t2_1_1 ++ n2 :: inorder t2_1_2) ++ n1 :: inorder t2_2) 
-											with (n0 :: inorder t2_1_1 ++ n2 :: inorder t2_1_2 ++ n1 :: inorder t2_2) in H2.
-										apply sorted_app with (l1:=n0::inorder t2_1_1) in H2. 
-											inversion H2. apply H4. 
-										congruence. 
-									rewrite <- app_assoc. reflexivity. 
-								SSSSSSCase "app_sorted 3". simpl in H2. apply cons_sorted in H2. rewrite <- app_assoc in H2. 
-									apply sorted_app in H2.
-										inversion H2.
-											inversion H5. apply H6. 
-										simpl. congruence.
-									SSSSCase "height2 = S n". destruct height2.
-										SSSSSCase "height2' = 0". simpl. apply app_sorted. 
-											SSSSSSCase "app_sorted 1". 
-												simpl. rewrite last_app_l. simpl in H2. apply sorted_app with (l1:=n0::inorder t2_1) in H2. 
-													inversion H2. inversion H5. apply H7. congruence. 
-											SSSSSSCase "app_sorted 2". simpl in H2. apply sorted_app with (l1:=n0::inorder t2_1) in H2. 
-												inversion H2. apply app_sorted. 
-													SSSSSSSCase "app_sorted 2_1". simpl. apply last_add. symmetry in Heqadd. 
-														apply ble_nat_true in Heqadd. assumption. assumption.
-													SSSSSSSCase "app_sorted 2_2". apply add_preserves_bst'. assumption. 
-													SSSSSSSCase "app_sorted 2_3". assumption.
-													congruence.
-											SSSSSSCase "app_sorted 3". simpl in H2. 
-												apply sorted_app with (l1:=n0::inorder t2_1)(l2:=n1::inorder t2_2) in H2. 
-													inversion H2.
-													inversion H5. apply H6. congruence.
-										SSSSSCase "height2' = S n'". destruct t2_1. 
-											SSSSSSCase "t2_1 Leaf". apply empty. 
-											SSSSSSCase "t2_1 Node".	simpl. apply app_sorted. 
-												SSSSSSSCase "app_sorted 1". simpl. rewrite last_app_l.
-													simpl in H2. rewrite <- app_assoc in H2. apply sorted_app with (l1:=n0::inorder t2_1_1) in H2.
-													inversion H2. inversion H5. apply H7. simpl. congruence.
-												SSSSSSSCase "app_sorted 2". apply app_sorted.
-													simpl. apply last_add. symmetry in Heqadd. apply ble_nat_true in Heqadd. omega. assumption.
-													apply add_preserves_bst'. assumption. simpl in H2. rewrite <- app_assoc in H2. 
-													apply sorted_app with (l1:=n0::inorder t2_1_1) in H2. inversion H2. inversion H5. assumption.
-													simpl. congruence.
-												SSSSSSSCase "app_sorted 3". simpl in H2. rewrite <- app_assoc in H2. 
-													apply sorted_app with (l1:=n0::inorder t2_1_1) in H2. inversion H2. inversion H5. assumption.
-													simpl. congruence.
-										SSCase "height1 = S n". destruct height1.
-												SSSCase "height1' = 0". simpl. apply app_sorted. 
-													SSSSCase "app_sorted 1". simpl. admit.
-													SSSSCase "app_sorted 2". admit.
-													SSSSCase "app_sorted 3". admit.
-												SSSCase "height1' = S n'". destruct height1. 
-													SSSSCase "height1'' = 0". simpl. admit.
-													SSSSCase "height1'' = S n''". destruct height1.
-														SSSSSCase "height1''' = 0". simpl. admit.
-														SSSSSCase "height1''' = S n'''". destruct height1. 
-															SSSSSSCase "height1'''' = 0".
-																remember (add n t1) as nt1. destruct nt1.
-																	SSSSSSSCase "nt1 Leaf". apply empty.
-																	SSSSSSSCase "nt1 Node".
-																		remember (height nt1_1 + 2 - height nt1_2) as height3. 
-																		destruct height3.
-																			(*height3 = 0*)simpl. apply app_sorted. 
-																				(*app_sorted 1*) simpl. admit.
-																				(*app_sorted 2*) admit.
-																				(*app_sorted 3*) admit.
-																			(*height3 = S n*)destruct height3.
-																				(*height3' = 0*)destruct nt1_2.
-																					(*nt1_2 = Leaf*)apply empty.
-																					(*nt1_2 = Node*)simpl. admit.
-																				(*height3' = S n'*)simpl. admit.
-															SSSSSSCase "height1'''' = S n''''".
-																simpl. apply app_sorted. 
-																	SSSSSSSCase "app_sorted 1". simpl. admit.
-																	SSSSSSSCase "app_sorted 2". admit.
-																	SSSSSSSCase "app_sorted 3". admit.
-			SCase "Add right tree".
-				simpl. remember (height t1 + 2 - height (add n t2)) as height4. destruct height4.
-					SSCase "height4 = 0". remember (add n t2) as nt2. destruct nt2.
-						SSSCase "nt2 = Leaf". apply empty.
-						SSSCase "nt2 = Node". 
-							remember (height nt2_1 + 2 - height nt2_2) as height5. destruct height5.
-								SSSSCase "height5 = 0". destruct nt2_1.
-									SSSSSCase "nt2_1 = Leaf". apply empty.
-									SSSSSCase "nt2_1 = Node". simpl. admit.
-								SSSSCase "height5 = S n". destruct height5.
-									SSSSSCase "height5' = 0". simpl. admit.
-									SSSSSCase "height5' = S n'". destruct nt2_1.
-										SSSSSSCase "nt2_1 = Leaf". apply empty.
-										SSSSSSCase "nt2_1 = Node". simpl. admit.
-					SSCase "height4 = S n". destruct height4.
-						SSSCase "height4' = 0". simpl. admit.
-						SSSCase "height4' = S n'". destruct height4.
-							SSSSCase "height4'' = 0". simpl. admit.
-							SSSSCase "height4'' = S n''". destruct height4.
-								SSSSSCase "height4''' = 0". simpl. admit.
-								SSSSSCase "height4''' = S n'''". destruct height4.
-									SSSSSSCase "height4'''' = 0". destruct t1.
-										SSSSSSSCase "t1 = Leaf". apply empty.
-										SSSSSSSCase "t1 = Node". remember (height t1_1 + 2 - height t1_2) as height6. destruct height6.
-											(*height6 = 0*) simpl. admit.
-											(*height6 = S n*)destruct height6.
-												(*height6' = 0*)destruct t1_2.
-													(*t1_2 = Leaf*)apply empty.
-													(*t1_2 = Node*)simpl. admit.
-												(*height6' = S n'*)simpl. admit.
-									SSSSSSCase "height4'''' = S n''''". simpl. admit.
-	congruence.	
-Qed.*)
-
-Theorem insert_preserves_balance: forall n t t',
-	t = insert n t' ->height t <= log2 (length (inorder t') + 1) + 1 = true.
-Proof. 
-	intros. induction t'.
-		Case "leaf". rewrite H. reflexivity.
-		Case "node". simpl in *. rewrite H. destruct t'1. destruct t'2. simpl. admit. simpl.
-
+	intros. unfold insert. rewrite <- balance_inorder. apply add_preserves_bst. assumption. 
 Qed.
